CoqCode/AppSubtyping.v
@@ -13,7 +13,7 @@ Proof.
   induction H; eauto.
   - exists A. unfold typ_stack. auto.
   - exists typ_top. auto.
-  - destruct IHappsub. rewrite H0.
+  - destruct IHappsub. rewrite H1.
     simpl. exists x. reflexivity.
 Qed.
 
@@ -24,14 +24,9 @@ Proof.
   induction S; intros.
   - constructor.
   - simpl. apply as_fun.
-    apply IHS.
+    + apply sub_reflexivity.
+    + apply IHS.
 Qed.
-
-(***
-succ ,, not 3
-
-Int |- (Int -> Int) & (Bool -> Bool) <: Int -> Int
-***)
 
 Lemma appsub_transitivity :
   forall (S1 S2 : arg) (A B C: typ),
@@ -48,86 +43,37 @@ Proof.
     constructor. constructor.
   - simpl in *.
     constructor.
-    apply IHappsub with B.
-    reflexivity. assumption.
-  - apply as_and_l with (E:=E).
+    + assumption.
     + apply IHappsub with B.
       reflexivity. assumption.
-    +
+  - apply as_and_l.
+    + apply IHappsub with B.
+      reflexivity. assumption.
 Admitted.
-(*     + *)
-(*   - apply as_and_r. *)
-(*     apply IHappsub with B. *)
-(*     reflexivity. *)
-(*     assumption. *)
-(* Qed. *)
 
 Lemma appsub_to_sub :
   forall (S : arg) (A B : typ),
-  appsub S A B /\ B = typ_top -> sub A B.
+  appsub S A B -> sub A B.
 Proof.
-  intros S A B [H1 H2].
-  induction H1; eauto; subst.
-  - apply sub_reflexivity.
-  - rewrite H2. constructor.
+  intros S A B H.
+  induction H; eauto.
+  apply sub_reflexivity.
 Qed.
+
 
 Lemma sub_to_appsub :
   forall (S : arg) (A B1 : typ),
-    sub A (typ_stack S B1) ->
-    exists B2 : typ, (appsub S A (typ_stack S B2) /\ (sub B2 B1)) \/ B2 = typ_top.
+    sub A (typ_stack S B1) -> not (toplike B1) ->
+    exists B2 : typ, (appsub S A (typ_stack S B2) /\ (sub B2 B1)).
 Proof.
-  intros S A B1 H.
-  dependent induction H; eauto.
-Qed.
-  (* - destruct S. *)
-  (*   simpl. exists typ_int. split. *)
-  (*   constructor. simpl in x. rewrite <- x. *)
-  (*   constructor. *)
-  (*   inversion x. *)
-  (* - destruct S; simpl in *; subst. *)
-  (*   exists A. split. constructor. constructor. *)
-  (*   inversion x. *)
-  (* - destruct S; simpl in *; subst. *)
-  (*   exists typ_top. split. *)
-  (*   constructor. constructor. assumption. *)
-  (*   inversion x; subst. *)
-  (*   pose proof (IHsub S B1) as IHsub'. *)
-  (*   assert (IHsub_help: typ_stack S B1 = typ_stack S B1). *)
-  (*   reflexivity. *)
-    (* (* (inversion x; subst. *) *) *) *)
-(*     pose proof (IHsub2 S B1) as IHsub2'. *)
-(*     assert (IHsub2_help: typ_stack S B1 = typ_stack S B1). *)
-(*     reflexivity. *)
-(*     apply IHsub2' in IHsub2_help. *)
-(*     destruct IHsub2_help. *)
-(*     exists x0. split. *)
-(*     constructor. assumption. *)
-(*     destruct H1 as [H11 H12]. *)
-(*     assumption. *)
-(*     destruct H1 as [H11 H12]. *)
-(*     assumption. *)
-(*   - destruct S; simpl in *; subst. *)
-(*     exists A. split. constructor. constructor. assumption. assumption. *)
-(*     inversion x. *)
-(*   - destruct S; simpl in *; subst. *)
-(*     exists (typ_and A B). split. constructor. apply sub_AndL. assumption. *)
-(*     pose proof (IHsub (cons t S) B1) as IHsub'. *)
-(*     assert(IHsub_help: typ_arrow t (typ_stack S B1) = typ_stack (t :: S) B1). *)
-(*     simpl. reflexivity. *)
-(*     apply IHsub' in IHsub_help. *)
-(*     destruct IHsub_help. *)
-(*     destruct H0 as [H01 H02]. *)
-(*     exists x. split. apply as_AndL. *)
-(*     simpl in H01. assumption. assumption. *)
-(*   - destruct S; simpl in *; subst. *)
-(*     exists (typ_and A B). split. constructor. apply sub_AndR. assumption. *)
-(*     pose proof (IHsub (cons t S) B1) as IHsub'. *)
-(*     assert(IHsub_help: typ_arrow t (typ_stack S B1) = typ_stack (t :: S) B1). *)
-(*     simpl. reflexivity. *)
-(*     apply IHsub' in IHsub_help. *)
-(*     destruct  IHsub_help. *)
-(*     destruct  H0 as [H01 H02]. *)
-(*     exists x. split. apply as_AndR. *)
-(*     simpl in H01. assumption. assumption. *)
-(* Qed. *)
+  intros S A B1 H1 H2.
+  dependent induction H1.
+  - destruct S.
+    simpl. exists typ_int. split.
+    constructor. simpl in x. rewrite <- x.
+    constructor.
+    inversion x.
+  - destruct S; simpl in *; subst.
+    exists A. split. constructor. constructor.
+    inversion x.
+Admitted.
